Back to working, with better group trait

ovn/src/lib.rs
@@ -5,10 +5,11 @@
 
 pub mod ovn_traits;
 
-pub mod ovn_group;
 pub mod ovn_secp256k1;
 pub mod ovn_z_89;
+pub mod ovn_group;
 
-pub mod ovn_zk_z_89;
-pub mod ovn_zk_secp256k1;
-pub mod ovn_zkgroup;
+// pub mod ovn_zk_secp256k1;
+// pub mod ovn_zk_z_89;
+// pub mod ovn_zkgroup;
+// pub mod ovn_zkgroup_specific;
