ovn/src/ovn_group.rs
@@ -13,24 +13,24 @@ pub use crate::ovn_traits::*;
 ////////////////////
 
 #[derive(Serialize, SchemaType, Clone, Copy)]
-pub struct SchnorrZKPCommit<Z: Z_Field, G: Group<Z>> {
-    pub schnorr_zkp_u: G::group_type,
-    pub schnorr_zkp_c: Z::field_type,
-    pub schnorr_zkp_z: Z::field_type,
+pub struct SchnorrZKPCommit<G: Group> {
+    pub schnorr_zkp_u: G,
+    pub schnorr_zkp_c: G::Z,
+    pub schnorr_zkp_z: G::Z,
 }
 
 /** Non-interactive Schnorr proof using Fiat-Shamir heuristics (RFC 8235) */
 // https://www.rfc-editor.org/rfc/rfc8235
 // https://crypto.stanford.edu/cs355/19sp/lec5.pdf
-pub fn schnorr_zkp<Z: Z_Field, G: Group<Z>>(
+pub fn schnorr_zkp<G: Group>(
     random: u32,
-    h: G::group_type,
-    x: Z::field_type,
-) -> SchnorrZKPCommit<Z, G> {
-    let r = Z::random_field_elem(random);
+    h: G,
+    x: G::Z,
+) -> SchnorrZKPCommit<G> {
+    let r = G::Z::random_field_elem(random);
     let u = G::g_pow(r);
     let c = G::hash(vec![G::g(), h, u]);
-    let z = Z::add(r, Z::mul(c, x));
+    let z = G::Z::add(r, G::Z::mul(c, x));
 
     return SchnorrZKPCommit {
         schnorr_zkp_u: u,
@@ -40,46 +40,46 @@ pub fn schnorr_zkp<Z: Z_Field, G: Group<Z>>(
 }
 
 // https://crypto.stanford.edu/cs355/19sp/lec5.pdf
-pub fn schnorr_zkp_validate<Z: Z_Field, G: Group<Z>>(
-    h: G::group_type,
-    pi: SchnorrZKPCommit<Z, G>,
+pub fn schnorr_zkp_validate<G: Group>(
+    h: G,
+    pi: SchnorrZKPCommit<G>,
 ) -> bool {
     pi.schnorr_zkp_c == G::hash(vec![G::g(), h, pi.schnorr_zkp_u])
         && G::g_pow(pi.schnorr_zkp_z) == G::prod(pi.schnorr_zkp_u, G::pow(h, pi.schnorr_zkp_c))
 }
 
 #[derive(Serialize, SchemaType, Clone, Copy)]
-pub struct OrZKPCommit<Z: Z_Field, G: Group<Z>> {
-    pub or_zkp_x: G::group_type,
-    pub or_zkp_y: G::group_type,
-    pub or_zkp_a1: G::group_type,
-    pub or_zkp_b1: G::group_type,
-    pub or_zkp_a2: G::group_type,
-    pub or_zkp_b2: G::group_type,
+pub struct OrZKPCommit<G: Group> {
+    pub or_zkp_x: G,
+    pub or_zkp_y: G,
+    pub or_zkp_a1: G,
+    pub or_zkp_b1: G,
+    pub or_zkp_a2: G,
+    pub or_zkp_b2: G,
 
-    pub or_zkp_c: Z::field_type,
+    pub or_zkp_c: G::Z,
 
-    pub or_zkp_d1: Z::field_type,
-    pub or_zkp_d2: Z::field_type,
+    pub or_zkp_d1: G::Z,
+    pub or_zkp_d2: G::Z,
 
-    pub or_zkp_r1: Z::field_type,
-    pub or_zkp_r2: Z::field_type,
+    pub or_zkp_r1: G::Z,
+    pub or_zkp_r2: G::Z,
 }
 
 /** Cramer, Damgård and Schoenmakers (CDS) technique */
-pub fn zkp_one_out_of_two<Z: Z_Field, G: Group<Z>>(
+pub fn zkp_one_out_of_two<G: Group>(
     random_w: u32,
     random_r: u32,
     random_d: u32,
-    h: G::group_type,
-    xi: Z::field_type,
+    h: G,
+    xi: G::Z,
     vi: bool,
-) -> OrZKPCommit<Z, G> {
-    let w = Z::random_field_elem(random_w);
+) -> OrZKPCommit<G> {
+    let w = G::Z::random_field_elem(random_w);
 
     if vi {
-        let r1 = Z::random_field_elem(random_r);
-        let d1 = Z::random_field_elem(random_d);
+        let r1 = G::Z::random_field_elem(random_r);
+        let d1 = G::Z::random_field_elem(random_d);
 
         let x = G::g_pow(xi);
         let y = G::prod(G::pow(h, xi), G::g());
@@ -92,8 +92,8 @@ pub fn zkp_one_out_of_two<Z: Z_Field, G: Group<Z>>(
 
         let c = G::hash(vec![x, y, a1, b1, a2, b2]);
 
-        let d2 = Z::sub(c, d1);
-        let r2 = Z::sub(w, Z::mul(xi, d2));
+        let d2 = G::Z::sub(c, d1);
+        let r2 = G::Z::sub(w, G::Z::mul(xi, d2));
 
         OrZKPCommit {
             or_zkp_x: x,
@@ -109,8 +109,8 @@ pub fn zkp_one_out_of_two<Z: Z_Field, G: Group<Z>>(
             or_zkp_r2: r2,
         }
     } else {
-        let r2 = Z::random_field_elem(random_r);
-        let d2 = Z::random_field_elem(random_d);
+        let r2 = G::Z::random_field_elem(random_r);
+        let d2 = G::Z::random_field_elem(random_d);
 
         let x = G::g_pow(xi);
         let y = G::pow(h, xi);
@@ -123,8 +123,8 @@ pub fn zkp_one_out_of_two<Z: Z_Field, G: Group<Z>>(
 
         let c = G::hash(vec![x, y, a1, b1, a2, b2]);
 
-        let d1 = Z::sub(c, d2);
-        let r1 = Z::sub(w, Z::mul(xi, d1));
+        let d1 = G::Z::sub(c, d2);
+        let r1 = G::Z::sub(w, G::Z::mul(xi, d1));
 
         OrZKPCommit {
             or_zkp_x: x,
@@ -143,9 +143,9 @@ pub fn zkp_one_out_of_two<Z: Z_Field, G: Group<Z>>(
 }
 
 // Anonymous voting by two-round public discussion
-pub fn zkp_one_out_of_two_validate<Z: Z_Field, G: Group<Z>>(
-    h: G::group_type,
-    zkp: OrZKPCommit<Z, G>,
+pub fn zkp_one_out_of_two_validate<G: Group>(
+    h: G,
+    zkp: OrZKPCommit<G>,
 ) -> bool {
     let c = G::hash(vec![
         zkp.or_zkp_x,
@@ -156,7 +156,7 @@ pub fn zkp_one_out_of_two_validate<Z: Z_Field, G: Group<Z>>(
         zkp.or_zkp_b2,
     ]); // TODO: add i
 
-    (c == Z::add(zkp.or_zkp_d1, zkp.or_zkp_d2)
+    (c == G::Z::add(zkp.or_zkp_d1, zkp.or_zkp_d2)
         && zkp.or_zkp_a1 == G::prod(G::g_pow(zkp.or_zkp_r1), G::pow(zkp.or_zkp_x, zkp.or_zkp_d1))
         && zkp.or_zkp_b1
             == G::prod(
@@ -171,13 +171,13 @@ pub fn zkp_one_out_of_two_validate<Z: Z_Field, G: Group<Z>>(
             ))
 }
 
-pub fn commit_to<Z: Z_Field, G: Group<Z>>(g_pow_xi_yi_vi: G::group_type) -> Z::field_type {
+pub fn commit_to<G: Group>(g_pow_xi_yi_vi: G) -> G::Z {
     G::hash(vec![g_pow_xi_yi_vi])
 }
 
-pub fn check_commitment<Z: Z_Field, G: Group<Z>>(
-    g_pow_xi_yi_vi: G::group_type,
-    commitment: Z::field_type,
+pub fn check_commitment<G: Group>(
+    g_pow_xi_yi_vi: G,
+    commitment: G::Z,
 ) -> bool {
     G::hash(vec![g_pow_xi_yi_vi]) == commitment
 }
@@ -185,34 +185,36 @@ pub fn check_commitment<Z: Z_Field, G: Group<Z>>(
 #[hax::contract_state(contract = "OVN")]
 // #[cfg_attr(not(feature = "hax_compilation"), contract_state(contract = "OVN"))]
 #[derive(Serialize, SchemaType, Clone, Copy)]
-pub struct OvnContractState<Z: Z_Field, G: Group<Z>, const n: usize> {
-    pub g_pow_xis: [G::group_type; n],
-    pub zkp_xis: [SchnorrZKPCommit<Z, G>; n],
+pub struct OvnContractState<G: Group, const n: usize> {
+    pub g_pow_xis: [G; n],
+    pub zkp_xis: [SchnorrZKPCommit<G>; n],
 
-    pub commit_vis: [Z::field_type; n],
+    pub commit_vis: [G::Z; n],
 
-    pub g_pow_xi_yi_vis: [G::group_type; n],
-    pub zkp_vis: [OrZKPCommit<Z, G>; n],
+    pub g_pow_xi_yi_vis: [G; n],
+    pub zkp_vis: [OrZKPCommit<G>; n],
 
     pub tally: u32,
+
+    pub round1 : [bool; n],
 }
 
 #[hax::init(contract = "OVN")]
 // #[cfg_attr(not(feature = "hax_compilation"), init(contract = "OVN"))]
-pub fn init_ovn_contract<Z: Z_Field, G: Group<Z>, const n: usize>(// _: &impl HasInitContext,
-) -> InitResult<OvnContractState<Z, G, n>> {
-    Ok(OvnContractState::<Z, G, n> {
+pub fn init_ovn_contract<G: Group, const n: usize>(// _: &impl HasInitContext,
+) -> InitResult<OvnContractState<G, n>> {
+    Ok(OvnContractState::<G, n> {
         g_pow_xis: [G::group_one(); n],
-        zkp_xis: [SchnorrZKPCommit::<Z, G> {
+        zkp_xis: [SchnorrZKPCommit::<G> {
             schnorr_zkp_u: G::group_one(),
-            schnorr_zkp_z: Z::field_zero(),
-            schnorr_zkp_c: Z::field_zero(),
+            schnorr_zkp_z: G::Z::field_zero(),
+            schnorr_zkp_c: G::Z::field_zero(),
         }; n],
 
-        commit_vis: [Z::field_zero(); n],
+        commit_vis: [G::Z::field_zero(); n],
 
         g_pow_xi_yi_vis: [G::group_one(); n],
-        zkp_vis: [OrZKPCommit::<Z, G> {
+        zkp_vis: [OrZKPCommit::<G> {
             or_zkp_x: G::group_one(),
             or_zkp_y: G::group_one(),
             or_zkp_a1: G::group_one(),
@@ -220,64 +222,67 @@ pub fn init_ovn_contract<Z: Z_Field, G: Group<Z>, const n: usize>(// _: &impl Ha
             or_zkp_a2: G::group_one(),
             or_zkp_b2: G::group_one(),
 
-            or_zkp_c: Z::field_zero(),
+            or_zkp_c: G::Z::field_zero(),
 
-            or_zkp_d1: Z::field_zero(),
-            or_zkp_d2: Z::field_zero(),
+            or_zkp_d1: G::Z::field_zero(),
+            or_zkp_d2: G::Z::field_zero(),
 
-            or_zkp_r1: Z::field_zero(),
-            or_zkp_r2: Z::field_zero(),
+            or_zkp_r1: G::Z::field_zero(),
+            or_zkp_r2: G::Z::field_zero(),
         }; n],
 
         tally: 0,
-    })
+
+        round1: [false; n],
+   })
 }
 
 /** Currently randomness needs to be injected */
-pub fn select_private_voting_key<Z: Z_Field>(random: u32) -> Z::field_type {
+pub fn select_private_voting_key<Z: Field>(random: u32) -> Z {
     Z::random_field_elem(random)
 }
 
 #[derive(Serialize, SchemaType)]
-pub struct RegisterParam<Z: Z_Field> {
+pub struct RegisterParam<Z: Field> {
     pub rp_i: u32,
-    pub rp_xi: Z::field_type,
+    pub rp_xi: Z,
     pub rp_zkp_random: u32,
 }
 
 /** Primary function in round 1 */
 #[hax::receive(contract = "OVN", name = "register", parameter = "RegisterParam")]
 // #[cfg_attr(not(feature = "hax_compilation"), receive(contract = "OVN", name = "register", parameter = "RegisterParam"))]
-pub fn register_vote<Z: Z_Field, G: Group<Z>, const n: usize, A: HasActions>(
+pub fn register_vote<G: Group, const n: usize, A: HasActions>(
     ctx: impl HasReceiveContext,
-    state: OvnContractState<Z, G, n>,
-) -> Result<(A, OvnContractState<Z, G, n>), ParseError> {
-    let params: RegisterParam<Z> = ctx.parameter_cursor().get()?;
+    state: OvnContractState<G, n>,
+) -> Result<(A, OvnContractState<G, n>), ParseError> {
+    let params: RegisterParam<G::Z> = ctx.parameter_cursor().get()?;
     let g_pow_xi = G::g_pow(params.rp_xi);
 
-    let zkp_xi = schnorr_zkp::<Z, G>(params.rp_zkp_random, g_pow_xi, params.rp_xi);
+    let zkp_xi = schnorr_zkp::<G>(params.rp_zkp_random, g_pow_xi, params.rp_xi);
 
     let mut register_vote_state_ret = state.clone();
     register_vote_state_ret.g_pow_xis[params.rp_i as usize] = g_pow_xi;
     register_vote_state_ret.zkp_xis[params.rp_i as usize] = zkp_xi;
+    register_vote_state_ret.round1[params.rp_i as usize] = true;
 
     Ok((A::accept(), register_vote_state_ret))
 }
 
 #[derive(Serialize, SchemaType)]
-pub struct CastVoteParam<Z: Z_Field> {
+pub struct CastVoteParam<Z: Field> {
     pub cvp_i: u32,
-    pub cvp_xi: Z::field_type,
+    pub cvp_xi: Z,
     pub cvp_zkp_random_w: u32,
     pub cvp_zkp_random_r: u32,
     pub cvp_zkp_random_d: u32,
     pub cvp_vote: bool,
 }
 
-pub fn compute_g_pow_yi<Z: Z_Field, G: Group<Z>, const n: usize>(
+pub fn compute_g_pow_yi<G: Group, const n: usize>(
     i: usize,
-    xis: [G::group_type; n],
-) -> G::group_type {
+    xis: [G; n],
+) -> G {
     let mut prod1 = G::group_one();
     for j in 0..i {
         prod1 = G::prod(prod1, xis[j]);
@@ -293,17 +298,17 @@ pub fn compute_g_pow_yi<Z: Z_Field, G: Group<Z>, const n: usize>(
     g_pow_yi
 }
 
-pub fn compute_group_element_for_vote<Z: Z_Field, G: Group<Z>>(
-    xi: Z::field_type,
+pub fn compute_group_element_for_vote<G: Group>(
+    xi: G::Z,
     vote: bool,
-    g_pow_yi: G::group_type,
-) -> G::group_type {
+    g_pow_yi: G,
+) -> G {
     G::prod(
         G::pow(g_pow_yi, xi),
         G::g_pow(if vote {
-            Z::field_one()
+            G::Z::field_one()
         } else {
-            Z::field_zero()
+            G::Z::field_zero()
         }),
     )
 }
@@ -311,22 +316,22 @@ pub fn compute_group_element_for_vote<Z: Z_Field, G: Group<Z>>(
 /** Commitment before round 2 */
 #[hax::receive(contract = "OVN", name = "commit_to_vote", parameter = "CastVoteParam")]
 // #[cfg_attr(not(feature = "hax_compilation"), receive(contract = "OVN", name = "commit_to_vote", parameter = "CastVoteParam"))]
-pub fn commit_to_vote<Z: Z_Field, G: Group<Z>, const n: usize, A: HasActions>(
+pub fn commit_to_vote<G: Group, const n: usize, A: HasActions>(
     ctx: impl HasReceiveContext,
-    state: OvnContractState<Z, G, n>,
-) -> Result<(A, OvnContractState<Z, G, n>), ParseError> {
-    let params: CastVoteParam<Z> = ctx.parameter_cursor().get()?;
+    state: OvnContractState<G, n>,
+) -> Result<(A, OvnContractState<G, n>), ParseError> {
+    let params: CastVoteParam<G::Z> = ctx.parameter_cursor().get()?;
 
     for i in 0..n {
-        if !schnorr_zkp_validate(state.g_pow_xis[i], state.zkp_xis[i]) {
+        if !schnorr_zkp_validate(state.g_pow_xis[i], state.zkp_xis[i]) || !state.round1[i] {
             return Err(ParseError {});
         }
     }
 
-    let g_pow_yi = compute_g_pow_yi::<Z, G, n>(params.cvp_i as usize, state.g_pow_xis);
+    let g_pow_yi = compute_g_pow_yi::<G, n>(params.cvp_i as usize, state.g_pow_xis);
     let g_pow_xi_yi_vi =
-        compute_group_element_for_vote::<Z, G>(params.cvp_xi, params.cvp_vote, g_pow_yi);
-    let commit_vi = commit_to::<Z, G>(g_pow_xi_yi_vi);
+        compute_group_element_for_vote::<G>(params.cvp_xi, params.cvp_vote, g_pow_yi);
+    let commit_vi = commit_to::<G>(g_pow_xi_yi_vi);
 
     let mut commit_to_vote_state_ret = state.clone();
     commit_to_vote_state_ret.commit_vis[params.cvp_i as usize] = commit_vi;
@@ -336,17 +341,17 @@ pub fn commit_to_vote<Z: Z_Field, G: Group<Z>, const n: usize, A: HasActions>(
 /** Primary function in round 2, also opens commitment */
 #[hax::receive(contract = "OVN", name = "cast_vote", parameter = "CastVoteParam")]
 // #[cfg_attr(not(feature = "hax_compilation"), receive(contract = "OVN", name = "cast_vote", parameter = "CastVoteParam"))]
-pub fn cast_vote<Z: Z_Field, G: Group<Z>, const n: usize, A: HasActions>(
+pub fn cast_vote<G: Group, const n: usize, A: HasActions>(
     ctx: impl HasReceiveContext,
-    state: OvnContractState<Z, G, n>,
-) -> Result<(A, OvnContractState<Z, G, n>), ParseError> {
-    let params: CastVoteParam<Z> = ctx.parameter_cursor().get()?;
+    state: OvnContractState<G, n>,
+) -> Result<(A, OvnContractState<G, n>), ParseError> {
+    let params: CastVoteParam<G::Z> = ctx.parameter_cursor().get()?;
 
-    let g_pow_yi = compute_g_pow_yi::<Z, G, n>(params.cvp_i as usize, state.g_pow_xis);
+    let g_pow_yi = compute_g_pow_yi::<G, n>(params.cvp_i as usize, state.g_pow_xis);
     let g_pow_xi_yi_vi =
-        compute_group_element_for_vote::<Z, G>(params.cvp_xi, params.cvp_vote, g_pow_yi);
+        compute_group_element_for_vote::<G>(params.cvp_xi, params.cvp_vote, g_pow_yi);
 
-    let zkp_vi = zkp_one_out_of_two::<Z, G>(
+    let zkp_vi = zkp_one_out_of_two::<G>(
         params.cvp_zkp_random_w,
         params.cvp_zkp_random_r,
         params.cvp_zkp_random_d,
@@ -367,16 +372,16 @@ pub struct TallyParameter {}
 #[hax::receive(contract = "OVN", name = "tally", parameter = "TallyParameter")]
 // #[cfg_attr(not(feature = "hax_compilation"), receive(contract = "OVN", name = "tally", parameter = "TallyParameter"))]
 /** Anyone can tally the votes */
-pub fn tally_votes<Z: Z_Field, G: Group<Z>, const n: usize, A: HasActions>(
+pub fn tally_votes<G: Group, const n: usize, A: HasActions>(
     _: impl HasReceiveContext,
-    state: OvnContractState<Z, G, n>,
-) -> Result<(A, OvnContractState<Z, G, n>), ParseError> {
+    state: OvnContractState<G, n>,
+) -> Result<(A, OvnContractState<G, n>), ParseError> {
     for i in 0..n {
-        let g_pow_yi = compute_g_pow_yi::<Z, G, n>(i as usize, state.g_pow_xis);
-        if !zkp_one_out_of_two_validate::<Z, G>(g_pow_yi, state.zkp_vis[i]) {
+        let g_pow_yi = compute_g_pow_yi::<G, n>(i as usize, state.g_pow_xis);
+        if !zkp_one_out_of_two_validate::<G>(g_pow_yi, state.zkp_vis[i]) {
             return Err(ParseError {});
         }
-        if !check_commitment::<Z, G>(state.g_pow_xi_yi_vis[i], state.commit_vis[i]) {
+        if !check_commitment::<G>(state.g_pow_xi_yi_vis[i], state.commit_vis[i]) {
             return Err(ParseError {});
         }
     }
@@ -387,14 +392,14 @@ pub fn tally_votes<Z: Z_Field, G: Group<Z>, const n: usize, A: HasActions>(
     }
 
     let mut tally = 0;
-    let mut curr = Z::field_zero();
+    let mut curr = G::Z::field_zero();
     for i in 0..n as u32 {
         // Should be while, but is bounded by n anyways!
         if G::g_pow(curr) == vote_result {
             tally = i;
         }
 
-        curr = Z::add(curr, Z::field_one());
+        curr = G::Z::add(curr, G::Z::field_one());
     }
 
     let mut tally_votes_state_ret = state.clone();
