ovn/src/ovn_traits.rs
@@ -10,40 +10,39 @@ use hax_lib_macros::*;
 
 #[exclude]
 use hacspec_concordium::*;
-#[exclude]
-use hacspec_concordium_derive::*;
+
 
 ////////////
 // Traits //
 ////////////
 
-pub trait Z_Field: core::marker::Copy {
-    type field_type: PartialEq + Eq + Clone + Copy + hacspec_concordium::Serialize;
+/** Interface for field implementation */
+pub trait Field: core::marker::Copy + PartialEq + Eq + Clone + Copy + hacspec_concordium::Serialize {
+    fn q() -> Self;
 
-    fn q() -> Self::field_type;
+    fn random_field_elem(random: u32) -> Self;
 
-    fn random_field_elem(random: u32) -> Self::field_type;
+    fn field_zero() -> Self;
+    fn field_one() -> Self;
 
-    fn field_zero() -> Self::field_type;
-    fn field_one() -> Self::field_type;
-
-    fn add(x: Self::field_type, y: Self::field_type) -> Self::field_type;
-    fn sub(x: Self::field_type, y: Self::field_type) -> Self::field_type;
-    fn mul(x: Self::field_type, y: Self::field_type) -> Self::field_type;
+    fn add(x: Self, y: Self) -> Self;
+    fn sub(x: Self, y: Self) -> Self;
+    fn mul(x: Self, y: Self) -> Self;
 }
 
 /** Interface for group implementation */
-pub trait Group<Z: Z_Field>: core::marker::Copy {
-    type group_type: PartialEq + Eq + Clone + Copy + hacspec_concordium::Serialize;
+pub trait Group: core::marker::Copy + PartialEq + Eq + Clone + Copy + hacspec_concordium::Serialize {
+    type Z : Field;
 
-    fn g() -> Self::group_type; // Generator (elemnent of group)
+    fn g() -> Self; // Generator (elemnent of group)
 
-    fn g_pow(x: Z::field_type) -> Self::group_type;
-    fn pow(g: Self::group_type, x: Z::field_type) -> Self::group_type; // TODO: Link with q
-    fn group_one() -> Self::group_type;
-    fn prod(x: Self::group_type, y: Self::group_type) -> Self::group_type;
-    fn inv(x: Self::group_type) -> Self::group_type;
-    fn div(x: Self::group_type, y: Self::group_type) -> Self::group_type;
+    fn g_pow(x: Self::Z) -> Self;
+    fn pow(g: Self, x: Self::Z) -> Self; // TODO: Link with q
+    fn group_one() -> Self;
+    fn prod(x: Self, y: Self) -> Self;
+    fn inv(x: Self) -> Self;
+    fn div(x: Self, y: Self) -> Self;
 
-    fn hash(x: Vec<Self::group_type>) -> Z::field_type;
+    fn hash(x: Vec<Self>) -> Self::Z;
 }
+
