ovn/src/ovn_zk_secp256k1.rs
@@ -6,14 +6,14 @@ use hacspec_concordium::*;
 #[exclude]
 use hacspec_concordium_derive::*;
 
-pub use group::{ff::Field, Group};
 pub use crate::ovn_zkgroup::*;
+pub use group::{ff::Field, Group};
 
 use hacspec_bip_340::{GroupTrait::*, Point, *};
 
 impl MGroup for Point {
     fn hash(inp: Vec<Self>) -> Self::Scalar {
-        return Self::Scalar::ONE // TODO
+        return Self::Scalar::ONE; // TODO
     }
 }
 
@@ -21,7 +21,7 @@ use bls12_381::*;
 
 impl MGroup for Gt {
     fn hash(inp: Vec<Self>) -> Self::Scalar {
-        return Self::Scalar::ONE // TODO
+        return Self::Scalar::ONE; // TODO
     }
 }
 // hacspec_concordium::Serial + hacspec_concordium::Deserial,
