ovn/tests/ovn_example.rs
@@ -26,48 +26,32 @@ pub use hacspec_ovn::ovn_group::*;
 pub use hacspec_ovn::ovn_secp256k1::*;
 pub use hacspec_ovn::ovn_z_89::*;
 
-#[test]
-pub fn schorr_zkp_correctness() {
-    fn test(random_x: u32, random_r: u32) -> bool {
-        type Z = z_89;
-        type G = g_z_89;
-
-        let x: u32 = Z::random_field_elem(random_x);
+#[cfg(test)]
+pub fn schnorr_zkp_correctness<G: Group>(random_x: u32, random_r: u32) -> bool {
+        let x: G::Z = G::Z::random_field_elem(random_x);
         let pow_x = G::g_pow(x);
 
-        let pi: SchnorrZKPCommit<Z, G> = schnorr_zkp(random_r, pow_x, x);
+        let pi: SchnorrZKPCommit<G> = schnorr_zkp(random_r, pow_x, x);
 
-        let valid = schnorr_zkp_validate::<Z, G>(pow_x, pi);
+        let valid = schnorr_zkp_validate::<G>(pow_x, pi);
         valid
-    }
+}
 
+pub fn schnorr_zkp_z_89_correctness() {
     QuickCheck::new()
         .tests(10000)
-        .quickcheck(test as fn(u32, u32) -> bool)
+        .quickcheck(schnorr_zkp_correctness::<g_z_89> as fn(u32, u32) -> bool)
 }
 
 #[test]
 pub fn schorr_zkp_secp256k1_correctness() {
-    fn test(random_x: u32, random_r: u32) -> bool {
-        type Z = Z_curve;
-        type G = Group_curve;
-
-        let x: Z_curve = Z::random_field_elem(random_x);
-        let pow_x = G::g_pow(x);
-
-        let pi: SchnorrZKPCommit<Z, G> = schnorr_zkp(random_r, pow_x, x);
-
-        let valid = schnorr_zkp_validate::<Z, G>(pow_x, pi);
-        valid
-    }
-
     QuickCheck::new()
         .tests(10)
-        .quickcheck(test as fn(u32, u32) -> bool)
+        .quickcheck(schnorr_zkp_correctness::<Group_curve> as fn(u32, u32) -> bool)
 }
 
 #[cfg(test)]
-pub fn or_zkp_correctness<Z: Z_Field, G: Group<Z>>(
+pub fn or_zkp_correctness<G: Group>(
     random_w: u32,
     random_r: u32,
     random_d: u32,
@@ -75,10 +59,10 @@ pub fn or_zkp_correctness<Z: Z_Field, G: Group<Z>>(
     random_x: u32,
     v: bool,
 ) -> bool {
-    let mut h = G::g_pow(Z::random_field_elem(random_h));
-    let x = Z::random_field_elem(random_x);
-    let pi: OrZKPCommit<Z, G> = zkp_one_out_of_two(random_w, random_r, random_d, h, x, v);
-    let valid = zkp_one_out_of_two_validate::<Z, G>(h, pi);
+    let mut h = G::g_pow(G::Z::random_field_elem(random_h));
+    let x = G::Z::random_field_elem(random_x);
+    let pi: OrZKPCommit<G> = zkp_one_out_of_two(random_w, random_r, random_d, h, x, v);
+    let valid = zkp_one_out_of_two_validate::<G>(h, pi);
     valid
 }
 
@@ -86,30 +70,30 @@ pub fn or_zkp_correctness<Z: Z_Field, G: Group<Z>>(
 pub fn or_zkp_correctness_z89() {
     QuickCheck::new()
         .tests(10000)
-        .quickcheck(or_zkp_correctness::<z_89, g_z_89> as fn(u32, u32, u32, u32, u32, bool) -> bool)
+        .quickcheck(or_zkp_correctness::<g_z_89> as fn(u32, u32, u32, u32, u32, bool) -> bool)
 }
 
 #[test]
 // TODO: Fix inverse opeation, should make this test parse
 pub fn or_zkp_secp256k1_correctness() {
     QuickCheck::new().tests(10).quickcheck(
-        or_zkp_correctness::<Z_curve, Group_curve> as fn(u32, u32, u32, u32, u32, bool) -> bool,
+        or_zkp_correctness::<Group_curve> as fn(u32, u32, u32, u32, u32, bool) -> bool,
     )
 }
 
 #[cfg(test)]
-pub fn sum_to_zero<Z: Z_Field, G: Group<Z>, const n: usize>() {
-    let mut xis: [Z::field_type; n] = [Z::field_zero(); n];
-    let mut g_pow_xis: [G::group_type; n] = [G::group_one(); n];
+pub fn sum_to_zero<G: Group, const n: usize>() {
+    let mut xis: [G::Z; n] = [G::Z::field_zero(); n];
+    let mut g_pow_xis: [G; n] = [G::group_one(); n];
     use rand::random;
     for i in 0..n {
-        xis[i] = Z::random_field_elem(random());
+        xis[i] = G::Z::random_field_elem(random());
         g_pow_xis[i] = G::g_pow(xis[i]);
     }
 
     let mut res = G::group_one();
     for i in 0..n {
-        let g_pow_yi = compute_g_pow_yi::<Z, G, n>(i, g_pow_xis);
+        let g_pow_yi = compute_g_pow_yi::<G, n>(i, g_pow_xis);
         res = G::prod(res, G::pow(g_pow_yi, xis[i]));
     }
 
@@ -118,18 +102,62 @@ pub fn sum_to_zero<Z: Z_Field, G: Group<Z>, const n: usize>() {
 
 #[test]
 pub fn sum_to_zero_z89() {
-    sum_to_zero::<z_89, g_z_89, 55>()
+    sum_to_zero::<g_z_89, 55>()
 }
 
 #[test]
 pub fn sum_to_zero_secp256k1() {
-    sum_to_zero::<Z_curve, Group_curve, 55>()
+    sum_to_zero::<Group_curve, 55>()
+}
+
+use rand::random;
+
+
+#[derive(Copy, Clone, hacspec_concordium::Serial, hacspec_concordium::Deserial)]
+pub struct ElemOfEach<G : Group> {
+    i : u32,
+    z : G::Z,
+    g : G,
 }
 
 #[cfg(test)]
-pub fn test_correctness<Z: Z_Field, G: Group<Z>, const n: usize, A: HasActions>(
+pub fn test_params_of_group<
+    G: Group,
+    A: HasActions,
+    >() {
+    // Setup the context
+    let mut ctx = hacspec_concordium::test_infrastructure::ReceiveContextTest::empty();
+    let parameter = ElemOfEach::<G> {
+        i: random(),
+        z: G::Z::random_field_elem(random()),
+        g: G::g_pow(G::Z::random_field_elem(random())),
+    };
+    let parameter_bytes = to_bytes(&parameter);
+    let ctx_params = ctx.clone().set_parameter(&parameter_bytes);
+    let param_back: Result<ElemOfEach<G>, ParseError> =
+        ctx_params.parameter_cursor().get();
+    assert!(param_back.is_ok());
+
+    let wu_param = param_back.unwrap();
+    assert!(wu_param.i == parameter.i);
+    assert!(wu_param.z == parameter.z);
+    assert!(wu_param.g == parameter.g);
+}
+
+#[test]
+pub fn test_params_of_group_z89() {
+    test_params_of_group::<g_z_89, hacspec_concordium::test_infrastructure::ActionsTree>()
+}
+
+#[test]
+pub fn test_params_of_group_secp256k1() {
+    test_params_of_group::<Group_curve, hacspec_concordium::test_infrastructure::ActionsTree>()
+}
+
+#[cfg(test)]
+pub fn test_correctness<G: Group, const n: usize, A: HasActions>(
     votes: [bool; n],
-    xis: [Z::field_type; n],
+    xis: [G::Z; n],
     rp_zkp_randoms: [u32; n],
     cvp_zkp_random_ws1: [u32; n],
     cvp_zkp_random_rs1: [u32; n],
@@ -141,22 +169,22 @@ pub fn test_correctness<Z: Z_Field, G: Group<Z>, const n: usize, A: HasActions>(
     // Setup the context
     let mut ctx = hacspec_concordium::test_infrastructure::ReceiveContextTest::empty();
 
-    let mut state: OvnContractState<Z, G, n> = init_ovn_contract().unwrap();
+    let mut state: OvnContractState<G, n> = init_ovn_contract().unwrap();
 
     for i in 0..n {
-        let parameter = RegisterParam::<Z> {
+        let parameter = RegisterParam::<G::Z> {
             rp_i: i as u32,
             rp_xi: xis[i],
             rp_zkp_random: rp_zkp_randoms[i],
         };
         let parameter_bytes = to_bytes(&parameter);
         (_, state) =
-            register_vote::<Z, G, n, A>(ctx.clone().set_parameter(&parameter_bytes), state)
+            register_vote::<G, n, A>(ctx.clone().set_parameter(&parameter_bytes), state)
                 .unwrap();
     }
 
     for i in 0..n {
-        let parameter = CastVoteParam::<Z> {
+        let parameter = CastVoteParam::<G::Z> {
             cvp_i: i as u32,
             cvp_xi: xis[i],
             cvp_zkp_random_w: cvp_zkp_random_ws1[i],
@@ -166,12 +194,12 @@ pub fn test_correctness<Z: Z_Field, G: Group<Z>, const n: usize, A: HasActions>(
         };
         let parameter_bytes = to_bytes(&parameter);
         (_, state) =
-            commit_to_vote::<Z, G, n, A>(ctx.clone().set_parameter(&parameter_bytes), state)
+            commit_to_vote::<G, n, A>(ctx.clone().set_parameter(&parameter_bytes), state)
                 .unwrap();
     }
 
     for i in 0..n {
-        let parameter = CastVoteParam::<Z> {
+        let parameter = CastVoteParam::<G::Z> {
             cvp_i: i as u32,
             cvp_xi: xis[i],
             cvp_zkp_random_w: cvp_zkp_random_ws2[i],
@@ -181,19 +209,19 @@ pub fn test_correctness<Z: Z_Field, G: Group<Z>, const n: usize, A: HasActions>(
         };
         let parameter_bytes = to_bytes(&parameter);
         (_, state) =
-            cast_vote::<Z, G, n, A>(ctx.clone().set_parameter(&parameter_bytes), state).unwrap();
+            cast_vote::<G, n, A>(ctx.clone().set_parameter(&parameter_bytes), state).unwrap();
     }
 
     let parameter = TallyParameter {};
     let parameter_bytes = to_bytes(&parameter);
     ctx = ctx.set_parameter(&parameter_bytes);
 
-    (_, state) = tally_votes::<Z, G, n, A>(ctx.clone(), state).unwrap();
+    (_, state) = tally_votes::<G, n, A>(ctx.clone(), state).unwrap();
 
     let mut count = 0u32;
     for v in votes {
         if v {
-            count = count + 1; // += 1 does not work correctly
+            count = count + 1;
         }
     }
 
@@ -202,10 +230,10 @@ pub fn test_correctness<Z: Z_Field, G: Group<Z>, const n: usize, A: HasActions>(
 }
 
 #[cfg(test)]
-fn randomized_full_test<Z: Z_Field, G: Group<Z>, const n: usize>() -> bool {
+fn randomized_full_test<G: Group, const n: usize>() -> bool {
     use rand::random;
     let mut votes: [bool; n] = [false; n];
-    let mut xis: [Z::field_type; n] = [Z::field_zero(); n];
+    let mut xis: [G::Z; n] = [G::Z::field_zero(); n];
     let mut rp_zkp_randoms: [u32; n] = [0; n];
     let mut cvp_zkp_random_ws1: [u32; n] = [0; n];
     let mut cvp_zkp_random_rs1: [u32; n] = [0; n];
@@ -217,7 +245,7 @@ fn randomized_full_test<Z: Z_Field, G: Group<Z>, const n: usize>() -> bool {
 
     for i in 0..n {
         votes[i] = random();
-        xis[i] = Z::random_field_elem(random());
+        xis[i] = G::Z::random_field_elem(random());
         rp_zkp_randoms[i] = random();
         cvp_zkp_random_ws1[i] = random();
         cvp_zkp_random_rs1[i] = random();
@@ -227,7 +255,7 @@ fn randomized_full_test<Z: Z_Field, G: Group<Z>, const n: usize>() -> bool {
         cvp_zkp_random_ds2[i] = random();
     }
 
-    test_correctness::<Z, G, n, hacspec_concordium::test_infrastructure::ActionsTree>(
+    test_correctness::<G, n, hacspec_concordium::test_infrastructure::ActionsTree>(
         votes,
         xis,
         rp_zkp_randoms,
@@ -245,13 +273,13 @@ fn randomized_full_test<Z: Z_Field, G: Group<Z>, const n: usize>() -> bool {
 fn test_full_z89() {
     QuickCheck::new()
         .tests(100)
-        .quickcheck(randomized_full_test::<z_89, g_z_89, 55> as fn() -> bool)
+        .quickcheck(randomized_full_test::<g_z_89, 55> as fn() -> bool)
 }
 
-// // #[concordium_test]
-// #[test]
-// fn test_full_secp256k1() {
-//     QuickCheck::new()
-//         .tests(1)
-//         .quickcheck(randomized_full_test::<Z_curve, Group_curve, 15> as fn() -> bool)
-// }
+// #[concordium_test]
+#[test]
+fn test_full_secp256k1() {
+    QuickCheck::new()
+        .tests(1)
+        .quickcheck(randomized_full_test::<Group_curve, 15> as fn() -> bool)
+}
